Address further PR comments
Rename ID.Algorithm() to ID.EncryptionSuite().
Change behavior to allow final frame to be as long as the frame length, instead of producing a 0-length final frame.
Make `EncryptRegularFrame`'s `length` parameter ghost, to allow it to be used in the method specification without needing to be passed at run time.
Add TODO in Streams.dfy.

src/SDK/AlgorithmSuite.dfy
@@ -14,8 +14,8 @@ module AlgorithmSuite {
 
   newtype ID = x | x in VALID_IDS witness 0x0014
   {
-    function method Algorithm(): EncryptionSuites.EncryptionSuite
-      ensures Algorithm().Valid()
+    function method EncryptionSuite(): EncryptionSuites.EncryptionSuite
+      ensures EncryptionSuite().Valid()
     {
       Suite[this].algorithm
     }
